src/QUIC.Secret.Buffer.fsti
@@ -42,7 +42,7 @@ val with_buffer_hide
       B.loc_disjoint (Ghost.reveal lin `B.loc_union` Ghost.reveal lout) (Ghost.reveal l `B.loc_union` B.loc_buffer bl `B.loc_union` B.loc_buffer bs `B.loc_union` B.loc_buffer br) /\
       B.live h bl /\ B.live h bs /\ B.live h br /\
       B.as_seq h bl == B.as_seq h0 (B.gsub b 0ul from) /\
-      Seq.seq_reveal (B.as_seq h bs) == B.as_seq h0 (B.gsub b from (to `U32.sub` from)) /\
+      B.as_seq h bs == Seq.seq_hide #Secret.U8 (B.as_seq h0 (B.gsub b from (to `U32.sub` from))) /\
       B.as_seq h br == B.as_seq h0 (B.gsub b to (B.len b `U32.sub` to))
     ))
     (ensures (fun h res h' ->
@@ -59,3 +59,37 @@ val with_buffer_hide
     B.modifies (Ghost.reveal lout `B.loc_union` (if U32.v x1 = U32.v x2 then B.loc_none else B.loc_buffer (B.gsub b x1 (x2 `U32.sub` x1))) `B.loc_union` (if U32.v x3 = U32.v x4 then B.loc_none else B.loc_buffer (B.gsub b (from `U32.add` x3) (x4 `U32.sub` x3))) `B.loc_union` (if U32.v x5 = U32.v x6 then B.loc_none else B.loc_buffer (B.gsub b (to `U32.add` x5) (x6 `U32.sub` x5)))) h h' /\
     post res (B.as_seq h' (B.gsub b 0ul from)) (B.as_seq h' (B.gsub b from (to `U32.sub` from))) (B.as_seq h' (B.gsub b to (B.len b `U32.sub` to))) h'
   ))
+
+(* Not secret-related, but very useful for footprints *)
+
+inline_for_extraction
+let buffer_update_strong
+  (#t: Type0)
+  (b: B.buffer t)
+  (i: U32.t { U32.v i < B.length b })
+  (v: t)
+: HST.Stack unit
+  (requires (fun h -> B.live h b))
+  (ensures (fun h _ h' ->
+    B.modifies (B.loc_buffer (B.gsub b i 1ul)) h h' /\
+    B.as_seq h' b `Seq.equal` Seq.upd (B.as_seq h b) (U32.v i) v
+  ))
+= let b' = B.sub b i 1ul in
+  let h = HST.get () in
+  B.upd b' 0ul v;
+  let h' = HST.get () in
+  let f
+    (j: nat { j < B.length b })
+  : Lemma
+    (Seq.index (B.as_seq h' b) j == Seq.index (Seq.upd (B.as_seq h b) (U32.v i) v) j)
+  = let (b_, j_) =
+      if j < U32.v i
+      then B.gsub b 0ul i, j
+      else if j = U32.v i
+      then B.gsub b i 1ul, 0
+      else B.gsub b (i `U32.add` 1ul) (B.len b `U32.sub` (i `U32.add` 1ul)), j - (U32.v i + 1)
+    in
+    assert (Seq.index (B.as_seq h b) j == Seq.index (B.as_seq h b_) j_);
+    assert (Seq.index (B.as_seq h' b) j == Seq.index (B.as_seq h' b_) j_)
+  in
+  Classical.forall_intro f
